src/Minimal.Loader.fst
@@ -1,0 +1,52 @@
+module Minimal.Loader
+
+open LowStar.BufferOps
+open Spec.Hash.Definitions
+open Hacl.Hash.Definitions
+open Lib.IntTypes
+
+open HWIface
+
+module I  = FStar.Integers
+module HI  = Lib.IntTypes
+
+module SHA2       = Hacl.Hash.SHA2
+module SHA1       = Hacl.Hash.SHA1
+module MD5        = Hacl.Hash.MD5
+module HMAC       = Hacl.HMAC
+module Ed25519    = Hacl.Ed25519
+// module Curve25519 = Hacl.Curve25519
+
+module B   = LowStar.Buffer
+module LB  = Lib.Buffer
+module M   = LowStar.Modifies
+module HS  = FStar.HyperStack
+module HST = FStar.HyperStack.ST
+module CString = C.String
+
+let header_len = 1ul
+
+let load_header
+  (_: unit)
+: HST.ST (header: header_t)
+  (requires fun h -> True)
+  (ensures fun h0 header h1 -> B.(
+    all_disjoint (get_header_loc_l header) /\
+    modifies loc_none h0 h1 /\
+    h1 `contains_header` header))
+=
+  let version = uint #U32 #PUB 1 in
+  let binary_size   = 100ul in
+  let binary_hash   = B.malloc HS.root (u8 0x00) digest_len in
+  let header_sig    = B.malloc HS.root (u8 0x00) 64ul in
+  let binary        = B.malloc HS.root (u8 0x00) binary_size in
+  let header_raw    = B.malloc HS.root (u8 0x00) header_len in
+  let header_pubkey = B.malloc HS.root (u8 0x00) 32ul in
+  { version     = version
+  ; binary_size = binary_size
+  ; binary_hash = binary_hash
+  ; header_sig  = header_sig
+  ; binary      = binary
+  ; header_raw  = header_raw
+  ; header_pubkey = header_pubkey}
+
